---
title: Exercise 4.26
author: Qi Ji (A0167793L)
date: 19th September 2018
...

\let\setminus\smallsetminus
\newcommand{\set}[1]{\left\{ #1 \right\}}
\newcommand{\sqbr}[1]{\left[ #1 \right]}
\newcommand{\pbr}[1]{\left( #1 \right)}
\newcommand{\ang}[1]{\left\langle #1 \right\rangle}
\newcommand{\N}{\mathbb{N}}
\renewcommand{\P}{\mathcal{P}}
\renewcommand{\vec}{\mathbf}
\newcommand{\dom}{\operatorname{dom}}
\newcommand{\ran}{\operatorname{ran}}
\renewcommand{\Im}{\operatorname{Im}}
\newcommand{\qed}{\hfill$\square$}
\newcommand{\qedd}{\quad$\square$}

> Let \(n,m,k\in\N\), prove the following directly from the definitions.

## 1. \(n+1 = S(n)\).
Proceed via induction on \(n\).

Base case.
:   \(0 + 1 = 1\) by definition of \(+\), and \(S(0) = 1\) by definition of \(1\).

Induction.
:   Suppose \(n + 1 = S(n)\), want \(S(n) + 1 = S(S(n))\).
\begin{align*}
    S(n) + 1 &= S(n + 1) \tag*{definition of $+$} \\
    &= S(S(n))  \tag*{inductive hypothesis \qedd}
\end{align*}

## 2. \(n + (m + k) = (n + m) + k\)
Induction on \(n\).

Base case.
:   \(0 + (m + k) = m + k\) by definition of \(+\). \((0 + m) + k = m + k\) also by definition of \(+\).

Induction.
:   Suppose \(n + (m + k) = (n + m) + k\), want \(S(n) + (m + k) = (S(n) + m) + k\). We have
\begin{align*}
    S(n) + (m + k) &= S(n + (m + k)) \tag*{by definition of $+$} \\
    &= S((n + m) + k)   \tag*{inductive hypothesis} \\
    &= S(n + m) + k     \tag*{definition of $+$} \\
    &= (S(n) + m) + k   \tag*{definition of $+$}
\end{align*}
The induction is complete.\qed

__Notation.__ Brackets can now be liberally omitted for equations containing \(+\).

## 3. \(n + m = m + n\)

__Lemma (plus 0).__ \(m = m + 0\) for any \(m\in \N\).

*Proof.*
Proceed by induction on \(m\).

Base case.
:   \(0 + 0 = 0\) by definition of \(+\).

Induction.
:   Suppose \(m = m + 0\), want \(S(m) = S(m) + 0\).

    \(S(m) + 0 = S(m + 0)\) by definition of \(+\), applying induction hypothesis, \(S(m + 0) = S(m)\).\qed

The lemma helps establish base case of part 3.

### Addition in \(\N\) is commutative.

*Proof.*
Proceed by induction on \(n\).

Base case.
:   \(0 + m = m\) by definition of \(+\), and \(m = m + 0\) by (plus 0), this establishes base case.

Induction.
:   Suppose \(n + m = m + n\), want \(S(n) + m = m + S(n)\).
\begin{align*}
    S(n) + m &= S(n + m) \tag*{by definition of $+$} \\
    &= S(m + n) \tag*{by inductive hypothesis} \\
    &= (m + n) + 1 \tag*{by part 1} \\
    &= m + (n + 1) \tag*{by part 2} \\
    &= m + S(n) \tag*{by part 1 \qedd}
\end{align*}

## 4. \(n + n = 2n\).

\begin{align*}
    2\cdot n &= S(S(0))\cdot n \tag*{definition of $2$} \\
    &= (S(0) \cdot n) + n \tag*{definition of $\cdot$} \\
    &= ((0 \cdot n) + n) + n \tag*{definition of $\cdot$} \\
    &= (0 + n) + n \tag*{definition of $\cdot$} \\
    &= n + n \tag*{definition of $+$ \qedd}
\end{align*}

\newpage

## 5. If \(2n = 2m\), then \(n = m\).

__Notation.__ For this part, let all implicit quantifiers range over \(\N\).

Using part 4, reformulate the statement to prove as
\[\forall n \sqbr{ \forall m \sqbr{ n + n = m + m \implies n = m }}. \]
Now we can proceed by induction on \(n\).

Base case.
:   Let \(m\) be arbitrary, need to show that \(0 + 0 = m + m\) implies \(0 = m\).

    Suppose we have \(m\) such that \(0 + 0 = 0 = m + m\).
    By exercise 4.15, we have either \(m = 0\) or \(\exists k\in m\subseteq\N\sqbr{S(k) = m}\).

    *   Case \(m = 0\) we are done.

    *   Case \(\exists k\in\N\sqbr{S(k) = m}\), then \(m + m = S(k) + S(k) = S(k + S(k)) = 0\), contradicting Peano axiom.

Induction step.
:   Suppose for \(k\), we have \(\forall j \sqbr{k + k = j + j \implies k = j}\).
    Want to show that \(\forall m\sqbr{S(k) + S(k) = m + m \implies S(k) = m}\).

    Let \(m\) be arbitrary, suppose we have \(S(k) + S(k) = m + m\),
    similarly by exercise 4.15, either \(m = 0\) or \(\exists j\in m\subseteq\N\sqbr{S(j) = m}\).
    Note that in the case \(m = 0\), we have \(S(k) + S(k) = S(k + S(k)) = 0\) which contradicts Peano axiom,
    so the latter statement has to hold.
    Then our assumption could be rewritten as
\begin{align*}
    S(k) + S(k) &= S(j) + S(j)  \\
    S(k + S(k)) &= S(j + S(j))  \tag*{definition of $+$} \\
    S(S(k) + k) &= S(S(j) + j)  \tag*{part 3} \\
    S(S(k + k)) &= S(S(j + j))  \tag*{definition of $+$} \\
    k + k &= j + j  \tag*{Peano axiom twice} \\
    k &= j  \tag*{induction hypothesis} \\
    S(k) &= S(j) \\
    S(k) &= m
\end{align*}
This completes the induction.\qed


\newpage

## 6. \(n\cdot(m + k) = n\cdot m + n\cdot k\)

Induction on \(n\).

Base case.
:   \(0\cdot (m+k) = 0\) by definition of \(\cdot\), and \(0\cdot m + 0\cdot k = 0 + 0 = 0\) by definitions of \(\cdot\) and \(+\).

Induction.
:   Suppose \(n\cdot(m+k) = n\cdot m + n\cdot k\), want to show \(S(n)\cdot(m+k) = S(n)\cdot m + S(n)\cdot k\).

    Evaluating LHS gives
\begin{align*}
    S(n) \cdot (m + k)
    &= n\cdot (m + k) + (m + k) \tag*{definition of $\cdot$} \\
    &= n\cdot m + n\cdot k + m + k \tag*{induction hypothesis} \\
    &= n\cdot m + m + n\cdot k + k \tag*{part 3} \\
    &= S(n)\cdot m + S(n)\cdot k    \tag*{definition of $+$ \qedd}
\end{align*}


Before we proceed, some right-sided properties of \(\cdot\) require demonstration.

__Lemma (multiply 0).__ \(n\cdot 0 = 0\).

*Proof.* Trivial induction.\qed

__Lemma (multiply 1).__ \(n\cdot 1 = n\).

*Proof.* Induction on \(n\).
Base case \(n = 0\) is trivial, suppose \(n\cdot 1 = n\), then
\begin{align*}
    S(n)\cdot 1 &= n\cdot 1 + 1 \tag*{definition of $\cdot$} \\
    &= n + 1 \tag*{induction hypothesis} \\
    &= S(n) \tag*{part 1 \qedd}
\end{align*}

__Corollary (multiply right successor).__ \(n\cdot S(m) = n\cdot m + n\).

*Proof.* \(n\cdot S(m) = n\cdot (m + 1) = n\cdot m + n\cdot 1 = n\cdot m + n\).\qed

\newpage

## 7. \(n\cdot (m\cdot k) = (n\cdot m)\cdot k\)

Induction on \(k\).

Base case.
:   \(n\cdot (m\cdot 0) = 0\) by two applications of (multiply 0), and \((n\cdot m)\cdot k = 0\) by 1 application of the same lemma.
This establishes base case.

Induction step.
:   Suppose \(n\cdot (m\cdot k) = (n\cdot m)\cdot k\), want to show \(n\cdot (m\cdot S(k)) = (n\cdot m)\cdot S(k)\).
\begin{align*}
    n\cdot (m\cdot S(k)) &= n\cdot (m\cdot k + m) \tag*{multiply right successor} \\
    &= n\cdot (m\cdot k) + n\cdot m \tag*{part 6} \\
    &= (n\cdot m)\cdot k + n\cdot m \tag*{induction hypothesis} \\
    &= (n\cdot m)\cdot S(k) \tag*{multiply right successor \qedd}
\end{align*}

## 8. \(n\cdot m = m\cdot n\)

Induction on \(n\).

Base case.
:   \(0 \cdot m = 0\) by definition of \(\cdot\), and \(m\cdot 0 = 0\) by multiply 0.

Induction step.
:   Suppose \(n\cdot m = m\cdot n\), need to show \(S(n)\cdot m = m\cdot S(n)\).
\begin{align*}
    S(n) \cdot m &= n\cdot m + m \tag*{definition of $\cdot$} \\
    &= m\cdot n + m \tag*{induction hypothesis} \\
    &= m\cdot S(n)  \tag*{multiply right successor \qedd}
\end{align*}
