---
title: MA2202S Tutorial 1
author: Qi Ji
date: Week 3
...

\let\setminus\smallsetminus
\newcommand{\set}[1]{\left\{\, #1 \,\right\}}
\newcommand{\abs}[1]{\left\lvert #1 \right\rvert}
\newcommand{\norm}[1]{\left\lVert #1 \right\rVert}
\newcommand{\floor}[1]{\left\lfloor #1 \right\rfloor}
\newcommand{\qed}{\hfill$\square$}
\newcommand{\tagQED}{\tag*{$\square$}}
\newcommand{\Z}{\mathbb{Z}}\newcommand{\Q}{\mathbb{Q}}\newcommand{\N}{\mathbb{N}}\newcommand{\R}{\mathbb{R}}
\newcommand{\lcm}{\operatorname{lcm}}

# Tutorial 1A {-}

# Prove application form of mathematical induction

Define \(S := \set{n\in\N: P(n)}\), trivial.

# 

>Given two nonzero integers \(x\) and \(y\).
>Suppose \(d \in\N\) such that \(d\mid x\) and \(d\mid y\), and \(d\) satisfies the following property
>\[\forall c\in\Z\setminus\set{0}.~ c\mid x \land c\mid y \implies c\mid d.\]
>Show that \(d = \gcd(x,y)\).

*Proof.*
Let \(d' := \gcd(x,y)\).
By definition of \(\gcd\), \(d'\Z = \set{ax + by: a,b\in\Z}\), so \(d'\mid x\) and \(d'\mid y\).
By hypothesis, \(d' \mid d\).

On the other hand, with Bézout's identity to write \(d' = ax + by\) for some \(a,b\in\Z\).
By hypothesis we have \(d\mid x\) and \(d\mid y\) hence \(d\mid d'\),
therefore \(d = d'\).

# Qn 1.56(iii) on page 54 in [R].

>i. Find \(d = \gcd ( 12327 , 2409)\) .
>ii. Find integers \(s\) and \(t\) with \(d = 12327 s + 2409 t\) .
>iii. Put the fraction \( 2409 / 12327\) in lowest terms.

i.  Papa Euclid
ii. Extended papa Euclid
iii. Divide by \(d\).

## Papa Euclid

Euclidean `gcd` implemented in Haskell,
```haskell
gcd :: Integral a => a -> a -> a
gcd a 0 = abs a
gcd a d = let r = a `mod` d in
              gcd d r
```
which gives
```
λ gcd 12327 2409
3
```

## Extended papa Euclid

To extend `gcd`, we need a function which for any \(a,d\in\Z\), calculates
\(\gcd(a,d)\) and \(c_1,c_2\in\Z\) such that \(c_1a + c_2d = \gcd(a,d)\).
We already know that \(\gcd(a,d) = \gcd(d,r)\) where \(a = qd + r\) by division algorithm.
Suppose (by recursion) we have \(\gcd(d,r) = xd + yr\), then
\begin{align*}
    \gcd(d,r)
    &= xd + yr \\
    &= xd + y(a - qd) \\
    &= ya + (x-qy)d
\end{align*}
Hence we can implement extended Euclidean algorithm as such
```haskell
-- returns (gcd a d, c1, c2)
eea :: Integral a => a -> a -> (a, a, a)
eea a 0 = (abs a, signum a, 0)
eea a d = let (q, r) = a `divMod` d
              (res, x, y) = eea d r in
              (res, y, x - q*y)
```
Which we can compute and verify as
```
λ eea 12327 2409
(3,299,-1530)
λ 299 * 12327 - 1530 * 2409
3
```

## Division by 3
is left as an exercise for the reader.

# Proposition 1.55 in [R].

> Suppose \[x = p_1^{e_1}p_2^{e_2}\cdots p_s^{e_s} \text{ and } y = p_1^{f_1} p_2^{f_2}\cdots p_s^{f_s}\]
> are prime factorisations of \(x,y \in \N\) respectively.
> Where \(p_1,\dots,p_s\) are distinct primes and \(e_i, f_j \geq 0\).

(i) \(x\mid y\) if and only if \(e_i \leq f_i\) for \(i = 1,\dots, s\).

    *Proof.* Suppose \(e_i \leq f_i\), divisibility is trivial, for
\[x \cdot p_1^{f_1 - e_1}p_2^{f_2 - e_2} \cdots p_s^{f_s - e_s} = y.\]

(ii) Can just whack with question 2.

#

>Suppose \(m_1,m_2,m_3\) are mutually coprime positive integers.
>Let \(r\in\Z\) such that \(m_1\mid r\), \(m_2\mid r\), \(m_3\mid r\).
>Show that \(m_1m_2m_3 \mid r\).

By Bézout's identity, there exists \(s,t\in\Z\) such that
\[s m_1 + t m_2 = 1.\]
Then because \(m_1 \mid r\) and \(m_2 \mid r\),
\begin{align*}
    s m_1r + t m_2r &= r \\
    s m_1m_2 \frac{r}{m_2} + t m_2 m_1 \frac{r}{m_1} &= r
\end{align*}
we have \(m_1m_2 \mid r\). (Exercise done)

We claim that \(\gcd(m_1m_2, m_3) = 1\).
Factorise those integers and use Question 4 to observe that prime factors of \(m_1\) and \(m_2\) do not appear in \(m_3\).
Apply above argument again to obtain conclusion.

# Let \(x_1,\dots,x_n\in\Z\), define \(I = \set{a_1x_1+a_2x_2+\dots+a_nx_n: a_1,\dots,a_n\in\Z}\).

__Base cases.__
When \(n=1\), it's trivial that

i.   \(I_1 = \set{a_1x_1 : a_1\in\Z} = x_1\Z\)
ii.  \(x_1\mid x_1\)
iii. Suppose \(c\ne 0\) and \(c\mid x_1\) then \(c\mid x_1\).

__Induction.__
Suppose results hold for \(n-1\), then

i.   \(I_n = \set{y + a_nx_n : y \in I_{n-1}, a_n \in\Z}\).
     From IH, we have \(I_{n-1} = d_{n-1}\Z\) for some poz int \(d_{n-1}\), so \[I_n = \set{ad_{n-1} + a_nx_n : a,a_n \in \Z } \]
     then we have \(I_n = d_n\Z\) where \(d_n = \gcd(d_{n-1}, x_n)\).

ii.  By IH \(d_{n-1} \mid x_1,\dots,x_{n-1}\), because \(d_n \mid d_{n-1}\), \(d_n\) also divides those guys.
Additionally it's clear by gcd that \(d_n \mid x_n\).

iii. Suppose \(c\ne 0\) and \(c\mid x_i\) for \(i\in\set{1,\dots,n}\), we have by induction hypothesis \(c\mid d_{n-1}\)
We also have \(c \mid x_n\), then by question 2, because \(d_n := \gcd(d_{n-1},x_n)\) we have \(c\mid d_n\).

# ED \(\implies\) PID
Let \((R,+,\cdot)\) be an Integral domain (no zero divisors), and let there be a division algorithm on it.

*Proof.*
Let \(I\) be any ideal, take the image \(N(I\setminus\set{0}) \subseteq \N\).
By well-ordering principle, we have an element \(a\in I\) such that \(N(a)\) is least in the image.
We claim that \(I = aR\).

\(aR \subseteq I\) is trivial, for \(a\in I\).
Suppose for a contradiction, \(I \supset aR\), then let \(x\in I\) such that \(x\notin aR\), then divide \(x\) by \(a\), we have
\[x = aq + r \text{ for some } q,r\in R\text{ with } N(r) \ne 0, N(r) < N(a)\]
then we have \(r = x + (-q)a \in I\) with \(N(r) < N(a)\) which raises a contradiction.

# \(p\)-adic memes.

i.  __Note.__ This guy is __not__ a vector space,
for let \(v\in \Z[\frac1p]_{>0}\),
\[(\underbrace{1+1+\dots+1}_{p\text{ times}})v = 0v \ne pv\]

    __Spanning.__ Let \(x\in \Z[\frac1p]_{>0}\), goal is to show that it can be expressed as a \(\Z/p\Z\) linear combination of vectors in \(\set{p^i : i\in\Z}\).
From definition, we have \(x = z_0 + z_2\frac1p + \dots + z_m \frac1{p^m}\) for some \(z_i\in\Z\), then simplify the expression as
\[ x = \frac{q}{p^m} \text{ for some }q\in\Z. \]
Because \(x>0\) and \(p>0\), it's necessary that \(q>0\), then we can iteratively divide \(q\) by \(p\), like such
\begin{align*}
    q   &= q_1p + r_1 \\
    q_1 &= q_2p + r_2 \\
    &\dots \\
    q_{k-1} &= q_kp + r_k \\
    q_k &= 0
\end{align*}
Where each \(r_i \in \Z/p\Z\),
the last line is the assertion that iteratively dividing by a positive integer by another fixed positive integer eventually gives \(0\), which is easy to see.
Then we can rewrite \(q\) as
\[q = \underbrace{q_kp^k}_0 + r_kp^{k-1} + \dots + r_2p + r_1.\]
Substitute expression into \(x = \frac{q}{p^m}\) gives result.

    __Linear Independence.__
Let \(I \subseteq \Z, \abs{I}<\infty\), \((c_i)_{i\in I} \subseteq \Z/p\Z\) such that
\[\sum_{i\in I} c_ip^i = 0.\]
Equivalently, let \(r = \min I, t = \max I\),
\[ c_rp^r + c_{r+1}p^{r+1} + \dots + c_tp^t = 0 \]
Without loss of generality, we can assume that \(r \geq 0\), for we could multiply
\(p^{-r}\) into equation otherwise.

    *Handwave.* By uniqueness of remainder, use iterated division by \(p\) to show that all the \(c_i\) are \(0\).

ii. \(p\)-adic norm
    1.  \(\norm{px} = \frac1p \norm{x}\).
        Expand.

    2.  \(\norm{xy} = \norm{x}\norm{y}\)
        Expand.

    2.  \(\norm{x+y} \leq \max\{ \norm{x}, \norm{y}\}\)
        Expand.

iii. Metric stuff

     I'm lazy...

----

# Tutorial 1B {-}

# LCM

From tutorial 1A we have
\[\gcd(x,y) = p_1^{m_1} p_2^{m_2}\cdots p_s^{m_s}\]
where each \(m_i = \min(e_i, f_i)\).

Then
\[\lcm(x,y) = p_1^{e_1+f_1-m_1}p_2^{e_2+f_2-m_2}\cdots p_s^{e_s+f_s-m_s} \]
and since \(\max(a,b) = a + b - \min(a,b)\), we're done.

# More LCM

i. Let \(d = \gcd(x,y)\), recall the definition \(l = \lcm(x,y) := xy/d\).
Since \(d\mid x\), \(y/d \in \Z\), therefore \(x\mid l\).
Symmetric argument shows \(y\mid l\).

ii. Factorise the damn thing and argue via prime factors, it becomes uncomfortably obvious.

# Computation.

## Solve \(3x \equiv 1 \pmod{8}\).

By computer,
```
λ eea 3 8
(1,3,-1)
```
so a solution is \(x=3\).

## Simultaneous congruence.

> Solve \(x\equiv 2\pmod{5}\) and \(3x\equiv 1\pmod{8}\).

First rewrite the second equation as \(x\equiv 3\pmod{8}\) (multiply by inverse of \(3\)).

__Chinese Remainder Theorem__
says that the solution is \(b'sm + btm'\) where \(\gcd(m,m') = sm + tm'\).
By computer again,
```
λ eea 5 8
(1,-3,2)
```
\(s = -3\) and \(t = 2\), so a solution is \(-13 \equiv 27 \pmod{40}\).
By Chinese Remainder Theorem all other solutions are of the form \(27 + 40n\) where \(n\in\Z\).

# Let \(a,b,m\in\Z\) with \(a>0, m>0\) and let \(d=\gcd(a,m)\).

> i. Show that \(ax \equiv b\pmod{m}\) has an integral solution \(x\) if and only if \(d\mid b\).

First write \(d = as + mt\) for \(s,t\in\Z\).

Suppose \(d\mid b\), let \(k = \frac{b}{d} \in\Z\),
then \(b = aks + tkm \equiv a(ks) \pmod{m}\).

Conversely suppose \(ax\equiv b \pmod{m}\) for some \(x\in\Z\).
Then \[ax + km = b \text{ for some } m\in\Z.\]
Since \(d\mid a\) and \(d\mid m\) we have \(d\mid b\).

> ii. If \(x\) and \(x'\) are both solutions to (i), show that
> \[x \equiv x' \pmod{\frac{m}{d}}.\]

We have \(ax \equiv ax' \equiv b \pmod{m}\).
Let \(k,k'\in\Z\), with \(k\ne k'\) (otherwise trivial) such that
\[ax + km = ax' + k'm = b.\]
Rearrangement yields
\[a(x-x') = (k'-k)m\]
By question 2, \(a(x-x') \mid \lcm(a,m) := \frac{am}{d}\).
Let \(k''\in\Z\) such that
\[a (x-x') \cdot k'' = \frac{am}{d}.\]
Cancel \(a\) for \(a\ne 0\) and we have \(x\equiv x'\pmod{\frac{m}{d}}\).

# Chinese remainder theorem on more equations.

> Let \(m_1,m_2,m_3\) be mutually coprime positive integers.
> Let \(b_1,b_2,b_3 \in\Z\).
>
> i.  Show that \begin{align*}
    x &\equiv b_1 \pmod{m_1} \\
    x &\equiv b_2 \pmod{m_2} \\
    x &\equiv b_3 \pmod{m_3}
\end{align*}
has a solution \(x\in\Z\).

By Chinese Remainder Theorem,
the first two equations gives us a solution class
\[ x \equiv s_1 \pmod{m_1m_2} \]
for some \(s_1\in\Z\).
By an argument used in tutorial 1A somewhere, \(\gcd(m_1m_2, m_3) = 1\) still,
so by Chinese remainder theorem, the congruence equations
\begin{align*}
    x &\equiv s_1 \pmod{m_1m_2} \\
    x &\equiv b_3 \pmod{m_3}
\end{align*}
has a solution, which is unique modulo \(m_1m_2m_3\).
Uniqueness comes from the 1A question.

# I'm damn stupid

> i.

Suppose
\begin{align*}
    x \equiv b_1 \pmod{m_1} \\
    x \equiv b_2 \pmod{m_2}
\end{align*}
has common solution \(x\in\Z\), then
\begin{align*}
    x + k_1m_1 &= b_1 \\
    x + k_2m_2 &= b_2
\end{align*}
rearrangement yields
\[ b_1 - b_2 = k_1m_1 - k_2m_2 \]
which shows that \(\gcd(m_1,m_2) \mid b_1 - b_2\).

Conversely suppose
\(\gcd(m_1,m_2) \mid b_1 - b_2\), then
without loss of generality (scaling factor), exists \(k_1, k_2\in\Z\)
such that
\begin{align*}
    k_1m_1 - k_2m_2 &= b_2 - b_1 \\
    x := k_1m_1 + b_1 &= k_2m_2 + b_2
\end{align*}
verify that \(x\) satisfies the equations.

> ii. If \(x, x'\) are solutions to (i), show that
>     \[x\equiv x' \pmod{\lcm(m_1, m_2)}.\]

Let
\begin{align*}
    x &= b_1 + k_1m_1 = b_2 + k_2m_2 \\
    x' &= b_1 + k_1'm_1 = b_2 + k_2'm_2
\end{align*}
then
\begin{align*}
    x - x' = (k_1 - k_1')m_1 = (k_2 - k_2') m_2
\end{align*}
Since \(m_1 \mid x - x'\) and \(m_2 \mid x - x'\) we have \(\lcm(m_1, m_2) \mid x - x'\) giving the conclusion.

# Gaussian Integers are Euclidean

Draw

# Gaussian Integers

* \(\pi \in \Z[i]\) is prime if for any \(a,b\in\Z[i]\), \(\pi \mid ab \implies \pi \mid a \lor \pi \mid b\).
* \(\iota \in \Z[i]\) is irreducible if \(\iota\) is not a unit (\(N(\iota) \ne 1\)) and \(\iota = xy \implies N(x) = 1 \lor N(y) = 1\).

## Prime \(\iff\) irreducible
We define \(\gcd\) to be in the first quadrant, with argument in \([0,\pi/2)\).
Define \(U := \set{1,i,-1,-i}\) be units of \(\Z[i]\).

Let \(p\in\Z[i]\) be prime.
Suppose \(p = ab \implies p \mid ab \implies p\mid a \lor p\mid b\).
Case \(p\mid a\), \[1 = \frac{a}{p}b \implies b \in U.\]
Symmetric argument for \(p\mid b\).

Let \(p\in\Z[i]\) be irreducible,
\[p=ab \implies a \in U \lor b \in U\]
Suppose \(p\mid xy\), goal: \(p\mid x\) or \(p\mid y\).
Let \(d = \gcd(p,x)\), clearly \(d\mid p\).
\[p = dp_1 \text{ for some }p_1\in\Z[i]\]
Because \(p\) irreducible, \(d \in pU\) or \(d \in U\).

* Case \(d = pi^{0,1,2,3}\), \(d\mid x\implies p\mid x\).
* Case \(d = 1 = ap + bx\) for some \(a,b\in\Z[i]\), then \[p \mid y = apy + b(xy)\]

# \(\Z[i]\) is factorial.

Existence of prime factorisation flows *exactly* like proof in
<https://blog.nus.edu.sg/2018ma2202s/2018/07/03/1-3-unique-factorization-domain-part-1/>
.

----

```
⣿⣿⣿⣿⣿⣿⡷⣯⢿⣿⣷⣻⢯⣿⡽⣻⢿⣿⣿⣿⣿⣿⣿⣿⣿⣿⣿⣿⣿⣿⣿⣿⣿⣿⣿⣇⠸⣿⣿⣆⠹⣿⣿⢾⣟⣯⣿⣿⣿⣿⣿⣿⣽⣻⣿⣿⣿⣿⣿⣿⣿⣿⣷⡌
⣿⣿⣿⣿⣿⣿⣻⣽⡿⣿⣎⠙⣿⣞⣷⡌⢻⣟⣿⣿⣿⣿⣿⣿⣿⣿⣿⣿⣿⣷⣿⣿⣿⣿⣿⣿⡄⠹⣿⣿⡆⠻⣿⣟⣯⡿⣽⡿⣿⣿⣿⣿⣽⡷⣯⣿⣿⣿⣿⣿⣿⣿⣿⣿
⣿⣿⣿⣿⣿⣿⣟⣷⣿⣿⣿⡀⠹⣟⣾⣟⣆⠹⣯⣿⣿⣿⣿⣿⣿⣿⣿⣿⣿⣿⣿⣿⣿⣿⣿⣿⡇⢠⡘⣿⣿⡄⠉⢿⣿⣽⡷⣿⣻⣿⣿⣿⣿⡝⣷⣯⢿⣿⣿⣿⣿⣿⣿⣿
⣿⣿⣿⣿⣿⣿⣯⢿⣾⢿⣿⡄⢄⠘⢿⣞⡿⣧⡈⢷⣿⣿⣿⣿⣿⣿⣿⣿⣿⣿⣿⣿⣿⣿⣿⣿⡇⢸⣧⠘⣿⣷⠈⣦⠙⢿⣽⣷⣻⣽⣿⣿⣿⣿⣌⢿⣯⢿⣿⣿⣿⣿⣿⣿
⣿⣿⣿⣿⣿⣿⣟⣯⣿⢿⣿⡆⢸⡷⡈⢻⡽⣷⡷⡄⠻⣽⣿⣿⡿⣿⣿⣿⣿⣿⣿⣷⣿⣿⣿⣿⣏⢰⣯⢷⠈⣿⡆⢹⢷⡌⠻⡾⢋⣱⣯⣿⣿⣿⣿⡆⢻⡿⣿⣿⣿⣿⡟⣿
⣿⣿⣿⣿⣿⣿⡎⣿⢾⡿⣿⡆⢸⣽⢻⣄⠹⣷⣟⣿⣄⠹⣟⣿⣿⣟⣿⣿⣿⣿⣿⣿⣽⣿⣿⣿⡇⢸⣯⣟⣧⠘⣷⠈⡯⠛⢀⡐⢾⣟⣷⣻⣿⣿⣿⡿⡌⢿⣻⣿⣿⣿⣿⡌
⣿⣿⣿⣿⣿⣿⣧⢸⡿⣟⣿⡇⢸⣯⣟⣮⢧⡈⢿⣞⡿⣦⠘⠏⣹⣿⣽⢿⣿⣿⣿⣿⣯⣿⣿⣿⡇⢸⣿⣿⣾⡆⠹⢀⣠⣾⣟⣷⡈⢿⣞⣯⢿⣿⣿⣿⢷⠘⣯⣿⣿⣿⣿⣷
⣿⣿⣿⣿⣿⣿⣿⡈⣿⢿⣽⡇⠘⠛⠛⠛⠓⠓⠈⠛⠛⠟⠇⢀⢿⣻⣿⣯⢿⣿⣿⣿⣷⢿⣿⣿⠁⣾⣿⣿⣿⣧⡄⠇⣹⣿⣾⣯⣿⡄⠻⣽⣯⢿⣻⣿⣿⡇⢹⣾⣿⣿⣿⣿
⣿⣿⣿⣿⣿⣿⣿⡇⢹⣿⡽⡇⢸⣿⣿⣿⣿⣿⣞⣆⠰⣶⣶⡄⢀⢻⡿⣯⣿⡽⣿⣿⣿⢯⣟⡿⢀⣿⣿⣿⣿⣿⣧⠐⣸⣿⣿⣷⣿⣿⣆⠹⣯⣿⣻⣿⣿⣿⢀⣿⢿⣿⣿⣿
⣿⣿⣿⣿⣿⣿⣿⣿⠘⣯⡿⡇⢸⣿⣿⣿⣿⣿⣿⣿⣧⡈⢿⣳⠘⡄⠻⣿⢾⣽⣟⡿⣿⢯⣿⡇⢸⣿⣿⣿⣿⣿⣿⡀⢾⣿⣿⣿⣿⣿⣿⣆⠹⣾⣷⣻⣿⡿⡇⢸⣿⣿⣿⣿
⣿⣿⣿⣿⣿⣿⣿⣿⡇⢹⣿⠇⢸⣿⣿⣿⣿⣿⣿⣿⣿⣷⣄⠻⡇⢹⣆⠹⣟⣾⣽⣻⣟⣿⣽⠁⣾⣿⣿⣿⣿⣿⣿⣇⣿⣿⠿⠛⠛⠉⠙⠋⢀⠁⢘⣯⣿⣿⣧⠘⣿⣿⣿⣿
⣿⣿⣿⣿⣿⣿⣿⣿⣿⡈⣿⡃⢼⣿⣿⣿⣿⣿⣿⣿⣿⣿⣿⣦⡙⠌⣿⣆⠘⣿⣞⡿⣞⡿⡞⢠⣿⣿⣿⣿⣿⡿⠛⠉⠁⢀⣀⣠⣤⣤⣶⣶⣶⡆⢻⣽⣞⡿⣷⠈⣿⣻⣿⣿
⣿⣿⣿⣿⣿⣿⣿⣿⡿⠃⠘⠁⠉⠉⠉⠉⠉⠉⠉⠉⠉⠙⠛⠛⢿⣄⢻⣿⣧⠘⢯⣟⡿⣽⠁⣾⣿⣿⣿⣿⣿⡃⢀⢀⠘⠛⠿⢿⣻⣟⣯⣽⣻⣵⡀⢿⣯⣟⣿⢀⣿⣽⣿⣿
⣿⣿⣿⣟⣿⣿⣿⣿⣶⣶⡆⢀⣿⣾⣿⣾⣷⣿⣶⠿⠚⠉⢀⢀⣤⣿⣷⣿⣿⣷⡈⢿⣻⢃⣼⣿⣿⣿⣿⣻⣿⣿⣿⡶⣦⣤⣄⣀⡀⠉⠛⠛⠷⣯⣳⠈⣾⡽⣾⢀⣿⢾⣿⣿
⣿⢿⣿⣿⣻⣿⣿⣿⣿⣿⡿⠐⣿⣿⣿⣿⠿⠋⠁⢀⢀⣤⣾⣿⣿⣿⣿⣿⣿⣿⣿⣌⣥⣾⡿⣿⣿⣷⣿⣿⢿⣷⣿⣿⣟⣾⣽⣳⢯⣟⣶⣦⣤⡾⣟⣦⠘⣿⢾⡁⢺⣿⣿⣿
⣿⣻⣿⣿⡷⣿⣿⣿⣿⣿⡗⣦⠸⡿⠋⠁⢀⢀⣠⣴⢿⣿⣽⣻⢽⣾⣟⣷⣿⣟⣿⣿⣿⣳⠿⣵⣧⣼⣿⣿⣿⣿⣿⣾⣿⣿⣿⣿⣿⣽⣳⣯⣿⣿⣿⣽⢀⢷⣻⠄⠘⣯⣿⣿
⣿⢷⣻⣿⣿⣷⣻⣿⣿⣿⡷⠛⣁⢀⣀⣤⣶⣿⣛⡿⣿⣮⣽⡻⣿⣮⣽⣻⢯⣿⣿⣿⣿⣿⣿⣿⣿⣿⣿⣿⣿⣿⣿⣿⣿⣿⣿⣿⣿⣿⣿⣿⣿⣿⣿⣯⢀⢸⣿⢀⡆⣿⣿⣿
⠸⣟⣯⣿⣿⣷⢿⣽⣿⣿⣷⣿⣷⣆⠹⣿⣶⣯⠿⣿⣶⣟⣻⢿⣷⣽⣻⣿⣿⣿⣿⣿⣿⣿⣿⣿⣿⣿⣿⣿⣿⣿⣿⣿⣿⣿⣿⣿⣿⣿⣿⣿⣿⣿⣿⣿⢀⣯⣟⢀⡇⢼⣿⣿
⣇⠹⣟⣾⣻⣿⣿⢾⡽⣿⣿⣿⣿⣿⣆⢹⣶⣿⣻⣷⣯⣟⣿⣿⣽⣿⣿⣿⣿⣿⣿⣿⣿⣿⣿⣿⣿⣿⣿⣿⣿⣿⣿⣿⣿⣿⣿⣿⣿⣿⣿⣿⣿⣿⣿⡿⢀⡿⡇⢸⡇⢸⣿⡇
⣿⣆⠹⣷⡻⣽⣿⣯⢿⣽⣻⣿⣿⣿⣿⣆⢻⣿⣿⣿⣿⣿⣿⣿⣿⣿⣿⣿⣿⣿⣿⣿⣿⣿⣿⣿⠛⢻⣿⣿⣿⣿⣿⣿⣿⣿⣿⣿⣿⣿⣿⣿⣿⣿⣿⠇⢸⣿⠇⣼⡇⢸⡿⢠
⡙⠾⣆⠹⣿⣦⠛⣿⢯⣷⢿⡽⣿⣿⣿⣿⣆⠻⣿⣿⣿⣿⣿⣿⣿⣿⣿⣿⣿⣿⣿⣿⣿⣿⣿⠃⠎⢸⣿⣿⣿⣿⣿⣿⣿⣿⣿⣿⣿⣿⣿⣿⣿⣿⠏⢀⣿⣾⣣⡿⡇⢸⢃⣾
⣿⣷⡌⢦⠙⣿⣿⣌⠻⣽⢯⣿⣽⣻⣿⣿⣿⣧⠩⢻⣿⣿⣿⣿⣿⣿⣿⣿⣿⣿⣿⣿⣿⣿⡏⢰⢣⠘⣿⣿⣿⣿⣿⣿⣿⣿⣿⣿⣿⣿⣿⣿⡿⠃⢀⢀⢿⣞⣷⢿⡇⠉⣼⣿
⣿⣽⣆⠹⣧⠘⣿⣿⡷⣌⠙⢷⣯⡷⣟⣿⣿⣿⣷⡀⡹⣿⣿⣿⣿⣿⣿⣿⣿⣿⣿⣿⣿⣿⣷⣈⠃⣸⣿⣿⣿⣿⣿⣿⣿⣿⣿⣿⣿⣿⣿⠟⢀⣴⡧⢀⠸⣿⡽⣿⢀⣾⣿⣿
⢻⣽⣿⡄⢻⣷⡈⢿⣿⣿⢧⢀⠙⢿⣻⡾⣽⣻⣿⣿⣄⠌⢿⣿⣿⣿⣿⣿⣿⣿⣿⣿⣿⣿⣿⣿⣿⣿⣿⣿⣿⣿⣿⣿⣿⣿⣿⣿⣿⠛⢁⣰⣾⣟⡿⢀⡄⢿⣟⣿⢀⣿⣿⣿
⡄⢿⣿⣷⢀⠹⣟⣆⠻⣿⣿⣆⢀⣀⠉⠻⣿⡽⣯⣿⣿⣷⣈⢻⣿⣿⣿⣿⣿⣿⣿⣿⣿⣿⣿⣿⣿⣿⣿⣿⣿⣿⣿⣿⣿⣿⡿⠋⢀⣠⠘⣯⣷⣿⡟⢀⢆⠸⣿⡟⢸⣿⣿⣿
⣷⡈⢿⣿⣇⢱⡘⢿⣷⣬⣙⠿⣧⠘⣆⢀⠈⠻⣷⣟⣾⢿⣿⣆⠹⣿⣿⣿⣿⣿⣿⣿⣿⣿⣿⣿⣿⣿⣿⣿⣿⣿⣿⣿⡿⠋⣠⡞⢡⣿⢀⣿⣿⣿⠇⡄⢸⡄⢻⡇⣼⣿⣿⣿
⣿⣷⡈⢿⣿⡆⢣⡀⠙⢾⣟⣿⣿⣷⡈⠂⠘⣦⡈⠿⣯⣿⢾⣿⣆⠙⠻⠿⠿⠿⠿⡿⣿⣿⣿⣿⣿⣿⣿⣿⣿⠿⠛⢋⣠⣾⡟⢠⣿⣿⢀⣿⣿⡟⢠⣿⢈⣧⠘⢠⣿⣿⣿⣿
⣿⣿⣿⣄⠻⣿⡄⢳⡄⢆⡙⠾⣽⣿⣿⣆⡀⢹⡷⣄⠙⢿⣿⡾⣿⣆⢀⡀⢀⢀⢀⢀⢀⢀⢀⢀⢀⢀⢀⢀⣀⣠⣴⡿⣯⠏⣠⣿⣿⡏⢸⣿⡿⢁⣿⣿⢀⣿⠆⢸⣿⣿⣿⣿
⣿⣿⣿⣿⣦⡙⣿⣆⢻⡌⢿⣶⢤⣉⣙⣿⣷⡀⠙⠽⠷⠄⠹⣿⣟⣿⣆⢙⣋⣤⣤⣤⣄⣀⢀⢀⢀⢀⣾⣿⣟⡷⣯⡿⢃⣼⣿⣿⣿⠇⣼⡟⣡⣿⣿⣿⢀⡿⢠⠈⣿⣿⣿⡟
⣿⣿⣿⣿⣿⣷⣮⣿⣿⣿⡌⠁⢤⣤⣤⣤⣬⣭⣴⣶⣶⣶⣆⠈⢻⣿⣿⣆⢻⣿⣿⣿⣿⣿⣿⣷⣶⣤⣌⣉⡘⠛⠻⠶⣿⣿⣿⣿⡟⣰⣫⣴⣿⣿⣿⣿⠄⣷⣿⠆⢻⣿⣿⡇

- ine
```
