---
title: MA2202S Tutorial 2
author: Qi Ji
date: Week 4
...

\let\setminus\smallsetminus
\newcommand{\set}[1]{\left\{\, #1 \,\right\}}
\newcommand{\abs}[1]{\left\lvert #1 \right\rvert}
\newcommand{\norm}[1]{\left\lVert #1 \right\rVert}
\newcommand{\floor}[1]{\left\lfloor #1 \right\rfloor}
\newcommand{\qed}{\hfill$\square$}
\newcommand{\tagQED}{\tag*{$\square$}}
\newcommand{\Z}{\mathbb{Z}}\newcommand{\Q}{\mathbb{Q}}\newcommand{\N}{\mathbb{N}}\newcommand{\R}{\mathbb{R}}\newcommand{\C}{\mathbb{C}}\newcommand{\F}{\mathbb{F}}
\let\oldphi\phi
\let\phi\varphi
\let\vec\mathbf

# Tutorial 2A {-}

# Show addition modulo \(p\) is associative.

Case-split every damn thing.

# Show that \(((\Z/p\Z)^\times, \star)\) forms an Abelian group.

> \(p\) is prime, and \(a \star b := r\) where \(r\) is the remainder when \(ab\) is divided by \(p\).

Closure
:   By division algorithm \(r \leq p-1\). Claim that \(r \ne 0\), that is \(p \nmid ab\).
For suppose not then \(p\mid a\) (or \(p\mid b\)) which implies \(p \leq a\) which makes no sense.

Commute
:   \(ab = ba\) so \(r_{ab} = r_{ba}\).

Assoc
:   Goal is \((ab \mod p) c \mod p = a (bc \mod p) \mod p\).
Probably easier to show that both are equal to \(abc \mod p\).
Let
\begin{align*}
ab &= q p + r_{ab} \\
bc &= q'p + r_{bc} \\
abc &= q''p + r
\end{align*}
Then we have
\begin{align*}
abc
&= (qp + r_{ab})c \\
&= qpc + r_{ab}\,c \\
&= a(q'p + r_{bc}) \\
&= aq'p + a\,r_{bc}
\end{align*}
By division algorithm 
\[ a\,r_{bc} \equiv r_{ab} c \equiv r \pmod{p}. \]
which entails \(a \star (b\star c) = (a\star b) \star c = r_{abc}\).

Identity
:   Trivial verification that \(a \star 1 = 1 \star a = a\).

Inverse
:   For each \(a \in (\Z/p\Z)^\times \), because \(a<p\) and \(p\) prime, by BÃ©zout's identity,
there exists \(x,y\in\Z\) such that
\[ ax = 1 - py \]
by division algorithm let \(x = qp + b\) for some \(q\in\Z, b\in(\Z/p\Z)^\times\), note \(b\ne 0\) otherwise substituting back into above equation yields \(p(aq + y) = 1\).
Now
\[ ab = 1 - py - aqp \]
which means \(a\star b = r_{ab} = 1\).

# Matrix stuff

> \[ G = \set{ A \in M_n(\R): A A^\top = I, \det(A) = 1} \]
> Show that \(G\) under matrix multiplication is a group.

__Lemma 3.0.__ \(G\) under matrix multiplication is a magma.

*Proof.*
For any \(A,B \in G\), we have \((AB)(AB)^\top = ABB^\top A^\top = AA^\top = I\).
Additionally, by multiplicativity of \(\det\), \(\det(AB) = \det(A)\det(B) = 1\).
\hfill$\square$

__Lemma 3.1.__ \(G\) under matrix multiplication is a semigroup.

*Proof.*
Refer to MA1101R for a proof that matrix multiplication is associative.
\hfill$\square$

__Lemma 3.2.__ \(G\) under matrix multiplication is a monoid.

*Proof.*
It is known that \(I\) is the identity under matrix multiplication.
\(G\) contains \(I\), for \(I I^\top = II = I\) and \(\det(I) = 1\).
\hfill$\square$

__Almost done.__ \(G\) under matrix multiplication is a group.

*Proof.*
It remains to show existence of inverse.
Let \(A\in G\), by characterising property of \(G\), we have \(A A^\top = I\),
from MA1101R we also have \(A^\top A = I\),
So we just need to show that \(A^\top \in G\).

* \(A^\top A^{\top\top} = A^\top A = I\), check.
* \(\det(A^\top) = \det(A) = 1\), check.
\hfill$\square$

# A binary group is Abelian.

Let \(a,b\in G\).
\begin{align*}
    e &= (ab)(ab)   \\
    e &= abab   \\
    a &= bab    \\
    ab &= ba    \tagQED
\end{align*}

# Pigeonhole principle.

> Let \((G, *)\) be a finite group.
> Show that for any \(x\in G\), there exists \(n \in\N\) such that \(x^n = e\).

Let \(x\in G\) be arbitrary, define the set-theoretic map \(\phi\) as
\begin{align*}
    \phi : \N &\to G \\
    n &\mapsto x^n
\end{align*}
As \(G\) is finite, by pigeonhole principle, there exists \(i, j\in\N\), \(i < j\) (WLOG) such that
\[\phi(i) = x^i = x^j = \phi(j).\]
Multiply by \(x^{-1}\) \(i\) times and we have \(e = x^{j-i}\).
\hfill$\square$

# \(n\times n\) multiplication table

Let \(\abs{G} = \set{x_1, x_2, \dots, x_n}\).

## row

Fix a row \(i\), means we fix \(x_i * -\).
To show that every element \(g \in G\) occurs exactly once in the row of multiplication table, we show that
for any \(g\in G\), there exists unique \(x_j \in G\) such that \(x_i * x_j = g\).
This is true because \(x_i^{-1}\) is unique so we just set \(x_j := x_i^{-1}g\).

Alternatively,
the claim is equivalent to the assertion that
the left-multiply map \[a \mapsto x_i * a\] is a permutation on the set of \(G\),
because it is a operator on a finite set with an inverse, namely \(b \mapsto x_i^{-1} * b\).

## column
is analogous.

# Farming

Too much work.

# \((\Z, +, \times)\) is __not__ a field.

Lack of multiplicative inverse.

----

# Tutorial 2B {-}

# \(\Z/p\Z\) is a field under addition and multiplication \(\mod p\).

<h2>TODO!!!</h2>

\newcommand{\H}{\mathbb{H}}
\newcommand{\conj}[1]{\overline{ #1 }}

# Hamiltonian

Rewrite the definition more succinctly as
\[ \H = \set{ \begin{pmatrix} a & b \\ -\conj{b} & \conj{a}\end{pmatrix} : a,b \in \C }.\]

## Real vector space
We have \(\H \subseteq \mathbb{M}_2(\C)\).
The set of \(2\times 2\) complex matrices already forms a complex vector space,
which means it also forms a real vector space, for \(\R\) is a subfield of \(\C\).
By eyeballing from the definition inspect that \(\H\) is indeed closed under \(+\) and scalar multiplication.
\hfill$\square$

## \((\H^\times, \times)\) forms a non-Abelian group.

Closure.
:   Let \(a,b,c,d\in\C\), we have
\[
\begin{pmatrix}
a & b \\
-\conj{b} & \conj{a}
\end{pmatrix}
\begin{pmatrix}
c & d \\
-\conj{d} & \conj{c}
\end{pmatrix}
=
\begin{pmatrix}
ac - b\conj{d} & ad+b\conj{c} \\
-c\conj{b}-\conj{ad} & \conj{ac}-\conj{b}d
\end{pmatrix}
\]
verify that RHS is in \(\H\).

Associative.
:   Follows from that of matrix multiplication.

Identity.
:   Trivial to see that \(I\in\H\).

Existence of inverse.
:   For any \(a,b\in\C\), let
\[A = \begin{pmatrix}
a & b \\
-\conj{b} & \conj{a}
\end{pmatrix}\]
computing determinant, get \(\det(A) = a\conj{a} + b\conj{b} = \abs{a}^2 + \abs{b}^2\).
Because the size is only \(2\times 2\), the inverse matrix of \(A\) is eyeballable as
\[ A^{-1} = \frac{1}{\abs{a}^2 + \abs{b}^2} \begin{pmatrix}
\conj{a} & \conj{b} \\
-b & a
\end{pmatrix} \]
observe that \(A^{-1} \in \H\).

Not Abelian.
:   Define
\[
A = \begin{pmatrix} i & i \\ i & -i\end{pmatrix} \quad
B = \begin{pmatrix} 0 & 1+i \\ -1+i & 0\end{pmatrix}
\]
and we have
\[
AB = \begin{pmatrix} -1-i & -1+i \\ 1+i & -1+i \end{pmatrix}
\ne
\begin{pmatrix} -1+i & 1-i \\ -1-i & -1-i \end{pmatrix}
=BA
\tagQED \]

## Distributivity

Follows from matrix multiplication.
Refer to MA1101R notes, as \(\R^n\) proof in there generalises.

# Square roots...

> Let \(G\) be a finite group which for every \(x\in G\),
> there exists \(y\in G\) such that \(x = y^2\).
> Prove that every element in \(G\) has a unique square root in \(G\).

Let \(G = \set{x_1,\dots,x_n}\).
We consider the map \(\phi\) defined as
\begin{align*}
    \phi : G &\to G\\
    x_i &\mapsto x_i^2
\end{align*}
Suppose there exists a non-unique square root, say \(x,y,z\in G\), such that \(y\ne z\) but \(\phi(y) = \phi(z) = x\).
This means that \(\phi\) is not injective which implies \(\phi\) is not surjective (operator on finite set).
So there exists an element \(x\in G\) where for all \(x_i \in G\), \(\phi(x_i) \ne x\).
This contradicts assumption that every \(x\in G\) has a square root.
\qed

Alternatively consider the multiplication table of \(G\), the assertion "every element has a unique square root"
is equivalent to the assertion that the diagonals of the multiplication table form a permutation of the elements in \(G\).

# \(\abs{G}\) is even, number of elements in \(G\) of order \(2\) is odd.

Let \(n = \abs{G}\).
Consider \(G \setminus \set{e}\), it has \(n-1\) elements.
Suppose for a contradiction that a even number of elements in \(G \setminus\set{e}\) are of order \(2\).
Then we have an odd number of elements that are not inverses of themselves.
This is a contradiction as each element has a unique inverse, and inverses can only come in pairs.
\qed

# Orbits

> \(G\) is a subset of \(\operatorname{End}(V)\) that is a group under matrix multiplication.
> Let \(\vec{v} \in V\) be a column vector.
> A \(G\)-orbit of \(\vec{v}\) is
> \[ G\vec{v} = \set{g\vec{v} \in V : g \in G}. \]

## If \(\vec{w} \in G\vec{v}\), then \(G\vec{w} = G\vec{v}\).

Since \(\vec{w} \in G\vec{v}\), there exists \(h\in G\) such that \(\vec{w} = h\vec{v}\).
Take \(g\vec{w} \in G\vec{w}\), then \(g\vec{w} = gh\vec{v} \in G\vec{v}\) for \(gh \in G\) too.
Similarly take \(g'\vec{v} \in G\vec{v}\), \(g'\vec{v} = g' h^{-1}\vec{w} \in G\vec{w}\).
\qed

## Show that \(G\)-orbits are disjointed, either \(G\vec{w} = G\vec{v}\) or \(G\vec{v} \cap G\vec{w} = \emptyset\).

By law of excluded middle, either \(\vec{w} \in G\vec{v}\) or \(\vec{w} \notin G\vec{v}\).
If former, we win by part 1.
Otherwise, suppose for a contradiction \(G\vec{v} \cap G\vec{w} \ne \emptyset\),
let \(\vec{u}\) inhabit that set. Then there exists \(h, h' \in G\) such that \(\vec{u} = h\vec{v} = h'\vec{w}\).
Then we have \(\vec{w} = h'^{-1} h\vec{v}\), which contradicts fact that \(\vec{w} \notin G\vec{v}\).
\qed

## Every vector \(\vec{v}\in V\) belongs to some \(G\)-orbit.

Take \(\vec{v}\in V\), we have \(\vec{v} = e\vec{v}\) so \(\vec{v} \in G\vec{v}\).
\qed

## Orbits form a partition.

Easily follows from (ii) and (iii).

# Exact
>\[ \set{e} \to K \xrightarrow{i} G \xrightarrow{\phi} H \to \set{e} \]
>If \((G,*)\) is a group, show that \((H,\star)\) is a group, then show that \((K,*)\) is a group.

__\(\star\) is closed.__
For any \(h_1, h_2 \in H\), choose \(g_1, g_2\) such that \(h_i = \phi(g_i)\),
then \(h_1 \star h_2 = \phi(g_1) \star \phi(g_2) = \phi(g_1 * g_2) \in H\).

__Associative.__
Let \(h_1, h_2, h_3 \in H\), choose \(g_1, g_2, g_3\) such that \(h_i = \phi(g_i)\).
\begin{align*}
    (h_1 \star h_2) \star h_3 &= \phi(g_1 * g_2)) \star \phi(g_3) \\
    &= \phi((g_1 * g_2) * g_3) \\
    &= \phi(g_1 * (g_2 * g_3)) \\
    &= h_1 \star \phi(g_2 * g_3) \\
    &= h_1 \star (h_2 \star h_3)
\end{align*}

__Identity and Inverse.__ Analogous argument shows that \(\phi(e)\) is actually identity in \(H\).

## \(K\) is a group. {-}

__Closure.__
Let \(k, k' \in K\), we have \(\phi(k) = \phi(k') = \phi(e)\), then
\begin{align*}
    \phi(k) \star \phi(k') &= \phi(e) \star \phi(e) \\
    \phi(kk') &= \phi(e)
\end{align*}

__Associativity__ follows.

__Existence of identity.__ follows as \(\phi(e) = \phi(e)\).

__Inverse.__ Take \(k \in K\), suffices to show that \(k^{-1} \in K\).
\begin{align*}
    \phi(kk^{-1}) &= \phi(e) \\
    \phi(e) \star \phi(k^{-1}) &= \phi(e) \\
    \phi(k^{-1}) &= \phi(e)
\end{align*}

# Linear algebra

Let
\[
\phi: \left(\F_{13}\right)^3 \xrightarrow{\ \simeq\ } \left(\F_{13}\right)^3
\]
be a group isomorphism

## Consider those as vector spaces, show that \(\phi\) is a linear transformation. (Invertible is free)
The operation on \((\F_{13})^3\) is coordinate-wise addition due to the definition of a product group, therefore
\(\phi\) preserving vector addition is also for free.

Observe that field operations in \(\F_{13}\) respects the law that
\[ ab = \underbrace{b + b + \dots + b}_{a \text{ times}} \]
then let \(v\in (\F_{13})^3, \alpha \in \F_{13}\),
\begin{align*}
    \phi(a v) &= \phi(\underbrace{v + v + \dots + v}_{a \text{ times}}) \\
    &= \underbrace{\phi v + \phi v + \dots + \phi v}_{a \text{ times}} \\
    &= a\, \phi v
\end{align*}

## Counting matrices
(This feels like Tan Kai Meng's MA2101S PYP)

Following hint, to count number of invertible \(3\times 3\) matrices,
we just have to choose \(3\) basis vectors.
Let
\[A = \left(\begin{array}{c|c|c}
v_1 & v_2 & v_3
\end{array}\right)\]

* For \(v_1\) choose anyone except zero vector, giving \(13^3 - 1\) ways,
* Choose \(v_2\) from anything except those in span of \(v_1\), giving \(13^3 - 13\) ways,
* Choose \(v_3\) from anything except those in spam of \(v_1\) and \(v_2\), giving \(13^3 - 13^2\) ways,

multiply everything to get answer which is \(9726417792\).
